refine: add arch-specific arch_valid_irq
On RISCV64 invalidIRQ falls within the range constraint of maxIRQ,
meaning to match the C we need to know valid IRQ caps in Haskell don't
hold invalidIRQ. Since invalidIRQ does not need explicit handling on
other architectures, we add arch_valid_irq as an interface constant to
valid_cap', and unfold its definition automatically within the Arch
locale.

This also clears up remaining Refine+CRefine breakage on RISCV64.

Signed-off-by: Rafal Kolanski <rafal.kolanski@proofcraft.systems>

proof/refine/RISCV64/ArchInvsDefs_H.thy
@@ -129,6 +129,13 @@ definition arch_cap'_fun_lift :: "(arch_capability \<Rightarrow> 'a) \<Rightarro
 
 lemmas arch_cap'_fun_lift_simps[simp] = arch_cap'_fun_lift_def[split_simps capability.split]
 
+(* on RISCV64, there is an invalid IRQ within the bound of maxIRQ *)
+definition arch_valid_irq :: "irq \<Rightarrow> bool" where
+  "arch_valid_irq irq \<equiv> irq \<le> maxIRQ \<and> irq \<noteq> irqInvalid"
+
+(* within the Arch locale, we want automatic expansion of the valid irq conditions *)
+lemmas [simp] = arch_valid_irq_def
+
 definition is_device_frame_cap' :: "capability \<Rightarrow> bool" where
   "is_device_frame_cap' cap \<equiv> case cap of ArchObjectCap (FrameCap _ _ _ dev _) \<Rightarrow> dev | _ \<Rightarrow> False"
 
